src/coding.lean
@@ -662,45 +662,23 @@ begin
   exact this,
 end
 
-theorem rpartrec.univ (α σ) [primcodable α] [primcodable σ] (f : β → option τ) :
-  (λ x, ⟦x.1⟧^f x.2 : ℕ × α →. σ) partrec_in (λ x, f x) :=
-begin
-  simp[univ],
-  let f0 := (λ (n : ℕ), option.map (λ (a : β), encode (f a)) (decode β n)),
-  have c₁ : (λ n, roption.of_option (f0 n)) partrec_in pfun.lift f,
-  { simp[f0],
-    have e : (λ (n : ℕ), roption.of_option (option.map (λ (a : β), encode (f a)) (decode β n))) =
-      (λ (n : ℕ), roption.bind (decode β n) (λ (a : β), some $ encode (f a))),
-    { funext a, cases decode β a; simp[(>>=), roption.of_option] },
-    rw e,
-    have := computable.encode.to_rcomp.comp (refl_in ↑f),
-    have := (computable.of_option (computable.decode)).to_rpart.bind (this.comp snd),
-    exact this },
-  have c₀ := (code.eval_partrec f0).comp 
-    (((primrec.of_nat code).comp primrec.fst).to_comp.to_rcomp.pair
-    (computable.encode.comp computable.snd).to_rcomp),
-  have c₂ := c₀.trans c₁,
-  have c₃ := computable.of_option computable.decode,
-  have := c₂.bind (c₃.to_rpart.comp snd),
-  exact this,
-end
-
-theorem evaln_sound {e} {f : β → τ} {x : α} {y : σ} {s : ℕ} :
+theorem evaln_sound {e} {f : β → option τ} {x : α} {y : σ} {s : ℕ} :
   ⟦e⟧^f [s] x = some y → ⟦e⟧^f x = some y := 
 by{ simp[univn, univ, roption.eq_some_iff], 
     exact λ s h e, ⟨s, code.evaln_sound h, e⟩ }
 
-theorem rpartrec_univ_iff {f : α →. σ} {g : β → τ} :
-  f partrec_in (g : β →. τ) ↔ ∃ e, ⟦e⟧^g = f :=
+theorem rpartrec_univ_iff {f : α →. σ} {g : β → option τ} :
+  f partrec_in (λ x, g x) ↔ ∃ e, ⟦e⟧^g = f :=
 begin
-  simp[univn, univ, rpartrec, nat.rpartrec.reducible, roption.eq_some_iff],
-  let g' := (λ n, (decode β n).map (λ a, (encode (g a)))),
-  have : (λ (n : ℕ), roption.bind (decode β n) (λ (a : β), some (encode (g a)))) =
+  simp[univn, univ, rpartrec, nat.rpartrec.reducible, roption.eq_some_iff], unfold_coes,
+  let g' := (λ n, (decode β n).bind (λ a, (g a).map encode)),
+  have : (λ n, (roption.of_option (decode β n)).bind (λ a, roption.map encode (roption.of_option (g a)))) =
     (λ x, g' x : ℕ →. ℕ) := funext (λ x, 
-  by { unfold_coes, simp[g'], cases decode β x; simp[roption.of_option, (>>=)] }),
+  by { unfold_coes, simp[g'], cases decode β x with v; simp[roption.of_option, (>>=)],
+       cases g v; simp[roption.of_option, (>>=)] }),
   simp [this], split,
   { assume h, rcases nat.rpartrec.code.exists_code_opt.mp h with ⟨c, hc⟩, 
-    refine ⟨encode c, funext $ λ a, _⟩, simp, unfold_coes, simp[roption.of_option,hc] },
+    refine ⟨encode c, funext $ λ a, _⟩, simp, simp[roption.of_option,hc] },
   { rintros ⟨e, he⟩, simp[←he, g'], 
     have c₀ := (code.eval_partrec g').comp 
       ((computable.const (of_nat code e)).to_rcomp.pair computable.encode.to_rcomp),
@@ -711,13 +689,20 @@ begin
     exact rpartrec.nat_iff.mp this }
 end
 
+theorem rpartrec_univ_iff_total {f : α →. σ} {g : β → τ} :
+  f partrec_in pfun.lift g ↔ ∃ e, ⟦e⟧^(λ x, some $ g x) = f :=
+by { rw ← rpartrec_univ_iff, simp[roption.of_option], refl }
+
 protected theorem cond {c : α → bool} {f : α →. σ} {g : α →. σ} {h : β → τ}
   (hc : c computable_in (h : β →. τ)) (hf : f partrec_in (h : β →. τ)) (hg : g partrec_in (h : β →. τ)) :
   (λ a, cond (c a) (f a) (g a)) partrec_in (h : β →. τ) :=
-let ⟨e, hf⟩ := rpartrec_univ_iff.1 hf,
-    ⟨i, hg⟩ := rpartrec_univ_iff.1 hg in
+let h' : β → option τ := (λ x, some (h x)) in
+have lf : f partrec_in (λ x, h' x), { simp[h'], exact hf },
+have lg : g partrec_in (λ x, h' x), { simp[h'], exact hg },
+let ⟨e, hf⟩ := rpartrec_univ_iff.1 lf,
+    ⟨i, hg⟩ := rpartrec_univ_iff.1 lg in
 begin
-  have c₀ := ((rpartrec.univ α σ h).comp $
+  have c₀ := ((rpartrec.univ α σ h').comp $
     (cond hc (const e) (const i)).pair id),
   simp at c₀,
   exact (c₀.of_eq $ λ x, by cases c x; simp[hg, hf] )
