src/incomparable_sets.lean
@@ -7,44 +7,76 @@ namespace t_reducible
 namespace Kleene_Post
 
 def extendable (l₀ l : list bool) (n e : ℕ) := (⟦e⟧^((l₀ ++ l).nth) n : roption bool).dom
+def extendable_ff (l₀ l : list bool) (n e : ℕ) := ⟦e⟧^((l₀ ++ l).nth) n = some ff
+def extendable_tt (l₀ l : list bool) (n e : ℕ) := ⟦e⟧^((l₀ ++ l).nth) n = some tt
 
 def extendable₀_le_0prime (l₀ : list bool) (n): 
   {e | ∃ l, extendable l₀ l n e} ≤ₜ ∅′ :=
 by sorry
 
-noncomputable mutual def L₀, L₁
-with L₀ : ℕ →. list bool
-| 0     := some []
-| (e+1) := do
-  σ₀ <- L₀ e,
-  σ₁ <- L₁ e,
-  decidable.cases_on (classical.dec $ ∃ l, extendable σ₁ l σ₀.length e)
-    (λ _, some $ ff :: σ₀)
-    (λ _, do
-    l₂ <- nat.rfind (λ l, chr $ extendable σ₁ (of_nat (list bool) l) σ₀ e),
-    
-    some $ σ₀)
-with L₁ : ℕ →. list bool
-| 0     := []
-| (e+1) := 
-  decidable.cases_on (classical.dec (extendable_ff (L₀ e) (L₁ e).length e))
-    (λ _, L₁ e)
-    (λ _, decidable.cases_on (classical.dec (extendable_tt (L₀ e) (L₁ e).length e))
-      (λ _, tt :: L₁ e)
-      (λ _, ff :: L₁ e))
+@[simp] theorem ε_operator_chr_Prop {β} [primcodable β] [inhabited β]
+  (p : β → Prop) (h : (ε_operator (chr p)).dom) :
+  p ((ε_operator (chr p)).get h) :=
+by { have := roption.get_mem h, have := ε_witness this, simp at this, exact this }
 
-def I₀ : set ℕ := {n | ∃ s, (L₀ s).nth n = tt}  
-def I₁ : set ℕ := {n | ∃ s, (L₁ s).nth n = tt}  
+
+theorem ε_operator_chr_Prop_iff {β} [primcodable β] [inhabited β]
+  (p : β → Prop) :
+  (∃ a, p a) ↔ (∃ a, a ∈ ε_operator (chr p)) :=
+by simp[←roption.dom_iff_mem]
+
+noncomputable def I : ℕ →. list bool × list bool
+| 0 := some ([], [])
+| (e+1) := do
+    σ  ← I e,
+    σ₁ ← cond (chr {e | ∃ l, extendable σ.2 l σ.1.length e} e)
+          (do l ← ε_operator (chr $ λ l, extendable σ.2 l σ.1.length e),
+              b ← (⟦e⟧^((σ.2 ++ l).nth) σ.1.length : roption bool),
+              some (σ.1 ++ [!b], σ.2 ++ l))
+          (some (σ.1 ++ [ff], σ.2)),
+    σ₂ ← cond (chr {e | ∃ l, extendable σ₁.1 l σ₁.2.length e} e)
+          (do l ← ε_operator (chr $ λ l, extendable σ₁.1 l σ₁.2.length e),
+              b ← (⟦e⟧^((σ₁.1 ++ l).nth) σ₁.2.length : roption bool),
+              some (σ₁.1 ++ l, σ₁.2 ++ [!b]))
+          (some (σ₁.1, σ₁.2 ++ [ff])),
+    some σ₂
+
+theorem I_defined (s) : (I s).dom :=
+begin
+  induction s with s0 ih; simp [I, bind_dom],
+  refine ⟨ih, _⟩,
+  cases c₀ : chr {e | ∃ l, extendable ((I s0).get ih).snd l ((I s0).get ih).fst.length e} s0; simp [roption.some],
+  { cases c₁ : chr {e | ∃ l, extendable (((I s0).get ih).fst ++ [ff]) l ((I s0).get ih).snd.length e} s0; simp [roption.some],
+    simp[set.set_of_app_iff] at c₀ c₁,
+    refine ⟨c₁, _⟩, simp[extendable] at c₁ ⊢, 
+    let p := λ l, (⟦s0⟧^((((I s0).get ih).fst ++ ff :: l).nth) ((I s0).get ih).snd.length : roption bool).dom,
+    have := ε_operator_chr_Prop p, exact this _ },
+  { simp[set.set_of_app_iff] at c₀,
+    let p := λ l, extendable ((I s0).get ih).snd l ((I s0).get ih).fst.length s0,
+    refine ⟨⟨c₀,_⟩, _⟩, 
+    { have := ε_operator_chr_Prop p, exact this _ },
+    { have : ∃ l, l ∈ ε_operator (chr p) := (ε_operator_chr_Prop_iff p).mp c₀,
+      rcases this with ⟨lb, hlb⟩, simp[p] at hlb, 
+      have hb := ε_witness hlb, simp only [chr_iff, extendable, roption.dom_iff_mem] at hb,
+      rcases hb with ⟨b, hb⟩,
+      simp[roption.eq_some_iff.mpr hlb, roption.eq_some_iff.mpr hb],
+      cases c₁ : chr {e | ∃ l, extendable (((I s0).get ih).fst ++ [!b]) l (((I s0).get ih).snd.length + lb.length) e} s0; simp[roption.some],
+      simp[set.set_of_app_iff] at c₁,
+      refine ⟨c₁, _⟩, simp[extendable] at c₁ ⊢, 
+      let p := λ (l : list bool), (⟦s0⟧^((((I s0).get ih).fst ++ !b :: l).nth) (((I s0).get ih).snd.length + lb.length)).dom,
+      have := ε_operator_chr_Prop p, simp[p] at this, exact this c₁ } }
+end
+
+def I₀ : set ℕ := {n | ∃ s, ((I s).get (I_defined s)).1.nth n = tt}  
+def I₁ : set ℕ := {n | ∃ s, ((I s).get (I_defined s)).2.nth n = tt}
 
 lemma inconparable01 : I₀ ≰ₜ I₁ :=
 begin
   assume h : I₀ ≤ₜ I₁,
   have l0 : ↑(chr I₀) partrec_in ↑(chr I₁) := classical_iff.mp h,
-  have : ∃ e, ⟦e⟧^(chr I₁) = ↑(chr I₀) := rpartrec.rpartrec_univ_iff.mp l0,
+  have : ∃ e, ⟦e⟧^(chr* I₁) = ↑(chr I₀) := rpartrec.rpartrec_univ_iff_total.mp l0,
   rcases this with ⟨e, he⟩,
-  cases classical.dec (extendable_ff (L₁ e) (L₀ e).length e) with F F;
-  cases classical.dec (extendable_tt (L₁ e) (L₀ e).length e) with T T,
-  have : L₀ e = 
+  sorry
 
 end
 
